\subsection{Method of Characteristics}
    \vspace{-1em}
    $$
        \frac{d}{dt}u(x(t),t) = \frac{\partial u}{\partial t} + \frac{d x(t)}{dt}\frac{\partial u}{\partial x} = \frac{\partial u}{\partial t} + a(x) \frac{\partial u}{\partial x} = 0
    $$
    Assume given $x(t)$ along which $u(x,t)$ is constant.
    \begin{align*}
        \frac{d}{dt} u(x(t),t) &= 0\\
        u_t + \dot{x}(t) \cdot u_x &= 0
    \end{align*}
    Since $u(x,t)$ also satisfies the LTE:
    $$
        \begin{cases}
            \dot{x}(t) &= a(x,t)\\
            x(0) &= x_0.
        \end{cases}
    $$
    $x(t)$ is called a \textit{characteristic curve}.\\
    From the initial assumption it follows, that:
    $$
        u(x(t),t) = u(x(0),0) = u(x_0,0) = u_0(x_0).
    $$
    \subsubsubsection{Example}
        \vspace{0.5em}
        $$
            \begin{cases}
                \dot{x}(t) = a, & a \in \mathbb{R}\\
                x(0) = x_0
            \end{cases}
        $$
        \begin{align*}
            x(t) &= at + x_0 \qquad \rightarrow x_0 = x(t) - at\\[0.5em]
            u(x,t) &= u_0(x_0) = u_0(x - at)
        \end{align*}