\subsection{Poisson Equation (PE)}
    \vspace{0.5em}
    \mathbox{
        -\Delta u = f
    }
\subsection{1D FD for PE}
    \vspace{-0.5em}
    $$
        \begin{cases}
            -u_{xx} &= f(x)\\
            \phantom{-}u(0) &= u(1) = 0
        \end{cases}
    $$
    \subsubsection{Solution}
        \vspace{-1em}
        \begin{align*}
            u(x) &= \int_0^1 G(x,y) \cdot f(y) \cdot dy\\
            G(x,y) &=
            \begin{cases}
                y(1-x)\quad 0 \leq y \leq x\\
                x(1-y)\quad x \leq y \leq 1
            \end{cases}
        \end{align*}
    \subsubsection{Numerics}
        \vspace{-0.7em}
        $$
            \Delta x = \frac{1}{N+1}
        $$
        \textbf{Finite Difference Method (FDM)}
        \begin{empheq}[box=\fbox]{align*}
            u''(x_i) &\approx \frac{u'(x_{i+ 1/2}) - u'(x_{i - 1/2})}{\Delta x}\\[0.5em]
                    &\approx \frac{u(x_{i+1}) - 2 u(x_i) + u(x_{i-1})}{\Delta x^2}
        \end{empheq}
        
        For the PE follows:
        $$
            - u(x_{i-1}) + 2 u(x_i) - u(x_{i+1}) = \Delta x^2 \cdot f(x_i)
        $$
        Which can be written as:
        \mathbox{A \cdot U = F}
        $$
            \!\!\!
            \begin{bmatrix}
                2 & -1 &  0 & 0 & \dots & 0 \\
                -1 &  2 & -1 & 0 & \dots & 0 \\
                \vdots & \ddots & \ddots & \ddots & \ddots & \vdots \\
                0 & \dots & 0 & -1 &  2 & -1 \\
                0 & \dots & 0 & 0 &  -1 &  2 
            \end{bmatrix}
            \!\!\!
            \begin{bmatrix}
                u(x_1) \\ u(x_2) \\ \vdots \\ \vdots\\ u(x_N)
            \end{bmatrix}
            \!\!
            = 
            \!\!
            \begin{bmatrix}
                f(x_1) \\ f(x_2) \\ \vdots \\ \vdots\\ f(x_N)
            \end{bmatrix}
            \!
            \Delta x^2
        $$
\subsection{2D FD for PE}
    \vspace{-0.5em}
    $$
        \begin{cases}
            -u_{xx} - u_{yy} &= f(x,y)\\
            \phantom{-}u\rvert_{\partial \Omega} &= 0
        \end{cases}
    $$
    $$
        \Delta x = \frac{1}{N_x+1} \qquad \Delta y = \frac{1}{N_y+1}
    $$
    \subsubsection{Solution for $N_x = N_y = N$}
        \vspace{0.5em}
        \mathbox{A \cdot U = F}
        $$
                \!\!\!
                \begin{bmatrix}
                    B & -\mathbb{I} &  0 & 0 & \dots & 0 \\
                    -\mathbb{I} &  B & -\mathbb{I} & 0 & \dots & 0 \\
                    \vdots & \ddots & \ddots & \ddots & \ddots & \vdots \\
                    0 & \dots & 0 & -\mathbb{I} &  B & -\mathbb{I} \\
                    0 & \dots & 0 & 0 &  -\mathbb{I} &  B 
                \end{bmatrix}
                \cdot U
                = 
                \!\!
                \begin{bmatrix}
                    f(x_1,y_1) \\ f(x_1,y_2) \\ \vdots \\ \vdots\\ f(x_N,y_N)
                \end{bmatrix}
                \!
                \Delta x^2
            $$
            $$
                B \vcentcolon= 
                \begin{bmatrix}
                    4 & -1 &  0 & 0 & \dots & 0 \\
                    -1 &  4 & -1 & 0 & \dots & 0 \\
                    \vdots & \ddots & \ddots & \ddots & \ddots & \vdots \\
                    0 & \dots & 0 & -1 &  4 & -1 \\
                    0 & \dots & 0 & 0 &  -1 &  4 
                \end{bmatrix}
                \in \mathbb{R}^{N \times N}
            $$
        \subsubsubsection{Lexicographical Ordering}
            \vspace{0.5em}
            $$
                (1,1) < \dots < (1,N_y) < \dots < (N_x,1) < \dots (N_x, N_y)
            $$
            \mathbox{
                u_{i,j}; \ (i,j) \quad \to \quad u_n;\ n = (i-1)\cdot N_y + j
            }